prove WPs and closure_interp are nonexpansive

theories/iris/language/cwp/def.v
@@ -1,4 +1,5 @@
 From iris.proofmode Require Import base proofmode classes.
+From iris.algebra Require Import list.
 From RichWasm.iris.language Require Import iris_wp_def lenient_wp logpred.
 Require Import RichWasm.iris.language.cwp.base.
 
@@ -10,9 +11,19 @@ Section def.
 
   Definition label_spec : Type := nat * (frame -> list value -> iProp Σ).
 
+  Definition label_specO : ofe := prodO (leibnizO nat) (leibnizO frame -n> leibnizO (list value) -n> iPropO Σ).
+
+  Definition label_ctxO : ofe := listO label_specO.
+
   Definition return_spec : Type := nat * (list value -> iProp Σ).
 
+  Definition return_specO : ofe := prodO (leibnizO nat) (leibnizO (list value) -n> iPropO Σ).
+
+  Definition return_ctxO : ofe := optionO return_specO.
+
   Definition fvs_pred : Type := frame -> list value -> iProp Σ.
+
+  Definition fvs_predO := leibnizO frame -n> leibnizO (list value) -n> iPropO Σ.
 
   Definition label_wand (l1 l2 : label_spec) : iProp Σ :=
     ⌜fst l1 = fst l2⌝ ∗ ∀ f vs, ⌜length vs = fst l1⌝ -∗ snd l1 f vs -∗ snd l2 f vs.
@@ -34,31 +45,125 @@ Section def.
   Definition fvs_combine (Φ : fvs_pred) (vs0 : list value) (f : frame) (vs : list value) : iProp Σ :=
     Φ f (vs0 ++ vs).
 
-  Definition cwp_post_br (L : list label_spec) (f : frame) (i : nat) (vh : valid_holed i) : iProp Σ :=
+  Program Definition coe_label_spec : label_specO -> label_spec :=
+    λ '(a, b), (a, λ f, b f).
+
+  Definition coe_label_ctx : label_ctxO -> list label_spec :=
+    fmap coe_label_spec.
+
+  Definition coe_return_ctx : return_ctxO -> option return_spec :=
+    λ R, match R with
+         | Some (n, R') => Some (n, λ v, R' v)
+         | None => None
+         end.
+
+  Definition cwp_post_br (f : frame) (i : nat) (vh : valid_holed i) (L : list label_spec) : iProp Σ :=
     match L !! (i - vh_depth vh) with
     | Some (n, P) => ∃ vs0 vs, ⌜get_base_l vh = vs0 ++ vs⌝ ∗ ⌜length vs = n⌝ ∗ P f vs
     | None => False
     end%I.
 
-  Definition cwp_post_ret (R : option return_spec) (svh : simple_valid_holed) : iProp Σ :=
+  (*
+  Lemma coe_label_ctx_ext (L L' : label_ctxO) (k : nat) n:
+    L ≡{n}≡ L' ->
+    ∀ (S S' : label_specO),
+      coe_label_ctx L !! k = Some (coe_label_spec S) ->
+      coe_label_ctx L' !! k = Some (coe_label_spec S') ->
+      S ≡{n}≡ S'.
+  *)
+
+  Program Definition cwp_post_br_ne (f : frame) (i : nat) (vh : valid_holed i) : label_ctxO -n> iProp Σ :=
+    λne L,
+      cwp_post_br f i vh (coe_label_ctx L).
+  Final Obligation.
+    intros * L L' Heq; cbn.
+    unfold coe_label_ctx, cwp_post_br.
+    rewrite !list_lookup_fmap.
+    set (k := i - vh_depth vh).
+    eapply (list_lookup_ne k) in Heq.
+    unfold lookup in *.
+    destruct Heq as [u v [Hn Ht] | ]; last done.
+    destruct u, v; solve_proper.
+  Qed.
+
+  Definition cwp_post_ret (svh : simple_valid_holed) (R : option return_spec) : iProp Σ :=
     match R with
     | Some (n, P) => ∃ vs0 vs, ⌜simple_get_base_l svh = vs0 ++ vs⌝ ∗ ⌜length vs = n⌝ ∗ P vs
     | None => False
     end%I.
 
-  Definition cwp_post_lp (L : list label_spec) (R : option return_spec) (Φ : fvs_pred) : logpred :=
-    {| lp_fr_inv _ := True;
-       lp_trap := True;
-       lp_val := Φ;
-       lp_br f i vh := cwp_post_br L f i vh;
-       lp_ret svh := cwp_post_ret R svh;
-       lp_host _ _ _ _ := False |}%I.
+  Program Definition cwp_post_ret_ne (svh : simple_valid_holed) : return_ctxO -n> iProp Σ :=
+    λne R, cwp_post_ret svh (coe_return_ctx R).
+  Final Obligation.
+    intros * R R' Heq; cbn.
+    destruct Heq as [x y [Heq1 Heq2] |]; [cbn | done].
+    destruct x, y; solve_proper.
+  Qed.
 
-  Definition cwp_wasm
-    (s : stuckness) (E : coPset) (es : list basic_instruction) (L : list label_spec)
-    (R : option return_spec) (Φ : fvs_pred) :
-    iProp Σ :=
+  Definition cwp_post_lp L R Φ : logpred :=
+      {| lp_fr_inv _ := True;
+         lp_trap := True;
+         lp_val f v := Φ f v;
+         lp_br f i vh := cwp_post_br f i vh L;
+         lp_ret svh := cwp_post_ret svh R;
+         lp_host _ _ _ _ := False |}%I.
+
+  Definition coe_fvs_pred : fvs_predO -> fvs_pred :=
+    λ Φ, λ f v, Φ f v.
+
+  Program Definition cwp_post_lp_ne : label_ctxO -n> return_ctxO -n> fvs_predO -n> logpredO :=
+    λne L R Φ, cwp_post_lp (coe_label_ctx L) (coe_return_ctx R) (coe_fvs_pred Φ).
+  Next Obligation.
+    intros * p q Hpq.
+    unfold coe_fvs_pred.
+    split; repeat match goal with
+           | |- _ /\ _ => split
+           end;
+      solve_proper.
+  Qed.
+  Next Obligation.
+    intros * R R' HR p; cbn.
+    unfold coe_fvs_pred.
+    split; repeat match goal with
+           | |- _ /\ _ => split
+           end; try solve_proper.
+    intros lh; cbn.
+    by eapply cwp_post_ret_ne.
+  Qed.
+  Final Obligation.
+    intros * L L' HL R p; cbn.
+    unfold coe_fvs_pred.
+    split; repeat match goal with
+           | |- _ /\ _ => split
+           end; try solve_proper.
+    intros *; cbn.
+    by eapply cwp_post_br_ne.
+  Qed.
+
+  Program Definition cwp_wasm (s : stuckness) (E : coPset) (es : list basic_instruction)
+                     L R Φ :=
     lenient_wp s E (to_e_list es) (cwp_post_lp L R Φ).
+
+  Program Definition cwp_wasm_ne (s : stuckness) (E : coPset) (es : list basic_instruction) :
+    label_ctxO -n> return_ctxO -n> fvs_predO -n> iPropO Σ :=
+    λne L R Φ,
+      lenient_wp s E (to_e_list es) (cwp_post_lp (coe_label_ctx L) (coe_return_ctx R) (coe_fvs_pred Φ)).
+  Next Obligation.
+    intros * p q Hpq.
+    eapply lenient_wp_ne.
+    by eapply (cwp_post_lp_ne L R).
+  Qed.
+  Next Obligation.
+    intros * R R' HR p; cbn.
+    eapply lenient_wp_ne.
+    by eapply (cwp_post_lp_ne L).
+  Qed.
+  Final Obligation.
+    intros * L L' HL R p; cbn.
+    eapply lenient_wp_ne.
+    by eapply cwp_post_lp_ne.
+  Qed.
+
 End def.
 
 Notation "'CWP' es @ s ; E 'UNDER' L ; R {{ Φ } }" :=
